fairness/fairness.v
@@ -1,11 +1,7 @@
-From trillium.program_logic Require Export adequacy.
 From stdpp Require Import option.
 From Paco Require Import paco1 paco2 pacotac.
-
-Require Import
-        Coq.Relations.Relation_Definitions
-        Coq.Relations.Relation_Operators.
-Require Import Coq.Arith.Wf_nat.
+From trillium.program_logic Require Export adequacy.
+From trillium.fairness Require Export inftraces.
 
 Record FairModel : Type := {
   fmstate:> Type;
@@ -19,8 +15,7 @@ Record FairModel : Type := {
   fmtrans: fmstate -> option fmrole -> fmstate -> Prop;
 
   live_roles: fmstate -> gset fmrole;
-  fm_live_spec:
-     forall s ρ s', fmtrans s (Some ρ) s' -> ρ ∈ live_roles s;
+  fm_live_spec: forall s ρ s', fmtrans s (Some ρ) s' -> ρ ∈ live_roles s;
 }.
 
 #[global] Existing Instance fmrole_eqdec.
@@ -30,9 +25,10 @@ Record FairModel : Type := {
 
 Section fairness.
   Context {Λ : language}.
+  Context {M: FairModel}.
   Context `{Countable (locale Λ)}.
 
-  Record LiveState (M: FairModel) := MkLiveState {
+  Record LiveState := MkLiveState {
     ls_under:> M.(fmstate);
 
     ls_fuel: gmap M.(fmrole) nat;
@@ -49,7 +45,7 @@ Section fairness.
   Arguments ls_mapping {_}.
   Arguments ls_same_doms {_}.
 
-  Lemma ls_mapping_dom M (m: LiveState M):
+  Lemma ls_mapping_dom (m: LiveState):
     M.(live_roles) m.(ls_under) ⊆ dom m.(ls_mapping).
   Proof. rewrite ls_same_doms. apply ls_fuel_dom. Qed.
 
@@ -58,6 +54,7 @@ Section fairness.
   | Silent_step: locale Λ -> FairLabel
   | Config_step: FairLabel
   .
+  Arguments FairLabel : clear implicits.
 
   Definition less (x y: option nat) :=
     match x, y with
@@ -65,9 +62,9 @@ Section fairness.
     | _, _ => False
     end.
 
-  Inductive must_decrease {M: FairModel} (ρ': M.(fmrole)) (oρ: option M.(fmrole)) (a b: LiveState M):
+  Inductive must_decrease (ρ': M.(fmrole)) (oρ: option M.(fmrole)) (a b: LiveState):
     olocale Λ -> Prop :=
-  | Same_tid tid (Hneqρ: Some ρ' ≠ oρ) (Hsametid: Some tid = (ls_mapping a) !! ρ'):
+  | Same_tid tid (Hneqρ: Some ρ' ≠ oρ) (Hsametid: Some tid = a.(ls_mapping) !! ρ'):
       must_decrease ρ' oρ a b (Some tid)
   | Change_tid otid (Hneqtid: a.(ls_mapping) !! ρ' ≠ b.(ls_mapping) !! ρ')
                (Hissome: is_Some (b.(ls_mapping) !! ρ')):
@@ -76,34 +73,18 @@ Section fairness.
     must_decrease ρ' oρ a b otid
   .
 
-  Definition oleq a b :=
-    match a, b with
-    | Some x, Some y => x ≤ y
-    | _, _ => False
-    end.
+  Definition fuel_decr (tid: olocale Λ) (oρ: option M.(fmrole))
+             (a b: LiveState) :=
+    ∀ ρ', ρ' ∈ dom a.(ls_fuel) -> ρ' ∈ dom b.(ls_fuel) →
+          must_decrease ρ' oρ a b tid ->
+          oless (b.(ls_fuel) !! ρ') (a.(ls_fuel) !! ρ').
 
-  Definition oless a b :=
-    match a, b with
-    | Some x, Some y => x < y
-    | _, _ => False
-    end.
-
-  Lemma oleq_oless a b: oless a b -> oleq a b.
-  Proof.
-    destruct a; destruct b=>//. unfold oless, oleq. lia.
-  Qed.
-
-  Definition fuel_decr {M: FairModel} (tid: olocale Λ) (oρ: option M.(fmrole)) (a b: LiveState M) :=
-    forall ρ', ρ' ∈ dom a.(ls_fuel) -> ρ' ∈ dom b.(ls_fuel) →
-          must_decrease ρ' oρ a b tid
-          -> oless (b.(ls_fuel) !! ρ') (a.(ls_fuel) !! ρ').
-
-  Definition fuel_must_not_incr {M: FairModel} oρ (a b: LiveState M) :=
+  Definition fuel_must_not_incr oρ (a b: LiveState) :=
     ∀ ρ', ρ' ∈ dom a.(ls_fuel) -> Some ρ' ≠ oρ ->
-          (oleq ((ls_fuel b) !! ρ') ((ls_fuel a) !! ρ')
+          (oleq (b.(ls_fuel) !! ρ') (a.(ls_fuel) !! ρ')
                 ∨ (ρ' ∉ dom b.(ls_fuel) ∧ ρ' ∉ M.(live_roles) a.(ls_under))).
 
-  Definition ls_trans {M} fuel_limit (a: LiveState M) ℓ (b: LiveState M): Prop :=
+  Definition ls_trans fuel_limit (a: LiveState) ℓ (b: LiveState): Prop :=
     match ℓ with
     | Take_step ρ tid =>
       M.(fmtrans) a (Some ρ) b
@@ -127,33 +108,32 @@ Section fairness.
       ∧ False (* TODO: add support for config steps later! *)
     end.
 
-  Definition fair_model_model M fuel_limit : Model := {|
-    mstate := LiveState M;
-    mlabel  := @FairLabel M.(fmrole);
-    mtrans := ls_trans fuel_limit;
+  Record LiveModel := {
+      lm_fl : M → nat;
+      lm_ls := LiveState;
+      lm_lbl := FairLabel M.(fmrole);
+      lm_ls_trans := ls_trans lm_fl;
+    }.
+  
+  Definition fair_model_model `(LM : LiveModel) : Model := {|
+    mstate := lm_ls LM;
+    mlabel := lm_lbl LM;
+    mtrans := lm_ls_trans LM;
   |}.
 
-  Record LiveModel (Λ: language) (M: FairModel) := {
-    fuel_limit : M -> nat;
-  }.
-
-  #[global] Arguments fuel_limit {_ _ _} _.
-
-  Definition live_model_to_model : forall M, LiveModel Λ M -> Model := λ M lm, fair_model_model M lm.(fuel_limit).
-  Coercion live_model_to_model : LiveModel >-> Model.
-
-  Definition tids_smaller {M: FairModel} (c : list (expr Λ)) (δ: LiveState M) :=
+  Definition tids_smaller (c : list (expr Λ)) (δ: LiveState) :=
     ∀ ρ ζ, δ.(ls_mapping) !! ρ = Some ζ -> is_Some (from_locale c ζ).
 
-  Program Definition initial_ls {M} {LM: LiveModel Λ M} (s0: M) (ζ0: locale Λ): LiveState M :=
+  Program Definition initial_ls `{LM: LiveModel} (s0: M) (ζ0: locale Λ)
+    : LM.(lm_ls) :=
     {| ls_under := s0;
-       ls_fuel := gset_to_gmap (LM.(fuel_limit) s0) (M.(live_roles) s0);
+       ls_fuel := gset_to_gmap (LM.(lm_fl) s0) (M.(live_roles) s0);
        ls_mapping := gset_to_gmap ζ0 (M.(live_roles) s0);
     |}.
-  Next Obligation. intros ????. apply reflexive_eq. rewrite dom_gset_to_gmap //. Qed.
-  Next Obligation. intros ????. apply reflexive_eq. rewrite !dom_gset_to_gmap //. Qed.
+  Next Obligation. intros ???. apply reflexive_eq. rewrite dom_gset_to_gmap //. Qed.
+  Next Obligation. intros ???. apply reflexive_eq. rewrite !dom_gset_to_gmap //. Qed.
 
-  Definition labels_match {M} (oζ : olocale Λ) (ℓ : @FairLabel (M.(fmrole))) :=
+  Definition labels_match `{LM:LiveModel} (oζ : olocale Λ) (ℓ : LM.(lm_lbl)) : Prop :=
     match oζ, ℓ with
     | None, Config_step => True
     | Some ζ, Silent_step ζ' => ζ = ζ'
@@ -161,228 +141,16 @@ Section fairness.
     | _, _ => False
     end.
 
-  Delimit Scope trace_scope with trace.
-
-  CoInductive trace (S L: Type) :=
-  | tr_singl (s: S)
-  | tr_cons (s: S) (ℓ: L) (r: trace S L).
-
-  Bind Scope trace_scope with trace.
-
-  Arguments tr_singl {_} {_}, _.
-  Arguments tr_cons {_} {_} _ _ _%trace.
-  Notation "⟨ s ⟩" := (tr_singl s) : trace_scope.
-  Notation "s -[ ℓ ]->  r" := (tr_cons s ℓ r) (at level 33) : trace_scope.
-  Open Scope trace.
-
-  Lemma trace_unfold_fold {S L} (tr: trace S L) :
-    tr = match tr with
-         | ⟨s⟩ => ⟨s⟩
-         | s -[ℓ]-> rest => s -[ℓ]-> rest
-         end.
-  Proof. destruct tr; trivial. Qed.
-
-  Definition trfirst {S L} (tr: trace S L): S :=
-    match tr with
-    | ⟨s⟩ => s
-    | s -[ℓ]-> r => s
-    end.
-
-  Section after.
-    Context {St L: Type}.
-
-    Fixpoint after (n: nat) (t: trace St L) : option (trace St L):=
-      match n with
-      | 0 => Some t
-      | Datatypes.S n =>
-        match t with
-        | ⟨ s ⟩ => None
-        | s -[ ℓ ]-> xs => after n xs
-        end
-      end.
-
-    Definition pred_at (tr: trace St L) (n: nat) (P: St -> option L -> Prop): Prop :=
-      match after n tr with
-      | None => False
-      | Some ⟨s⟩ => P s None
-      | Some (s -[ℓ]-> _) => P s (Some ℓ)
-      end.
-
-    Lemma after_sum m: forall k (tr: trace St L),
-        after (k+m) tr =
-        match after m tr with
-        | None => None
-        | Some tr' => after k tr'
-        end.
-    Proof.
-      induction m.
-      - intros k tr. by have ->: k+0=k by lia.
-      - intros k tr. simpl.
-        have -> /=: (k + S m) = S (k+m) by lia.
-        destruct tr as [s|s l r]; simpl; auto.
-    Qed.
-
-    Lemma after_sum' m: forall k (tr: trace St L),
-        after (k+m) tr =
-        match after k tr with
-        | None => None
-        | Some tr' => after m tr'
-        end.
-    Proof. intros. rewrite Nat.add_comm. apply after_sum. Qed.
-
-    Lemma pred_at_sum P n m tr:
-      pred_at tr (n + m) P <->
-      match after n tr with
-      | None => False
-      | Some tr' => pred_at tr' m P
-      end.
-    Proof.
-      rewrite /pred_at after_sum'.
-        by destruct (after n tr).
-    Qed.
-
-    Lemma pred_at_sum' P n m tr:
-      pred_at tr (n + m) P <->
-      match after m tr with
-      | None => False
-      | Some tr' => pred_at tr' n P
-      end.
-    Proof.
-      rewrite /pred_at after_sum.
-        by destruct (after m tr).
-    Qed.
-
-    Lemma pred_at_0 s ℓ r P:
-      pred_at (s -[ℓ]-> r) 0 P <-> P s (Some ℓ).
-    Proof. by unfold pred_at. Qed.
-
-    Lemma pred_at_S s ℓ r n P:
-      pred_at (s -[ℓ]-> r) (S n) P <-> pred_at r n P.
-    Proof. by unfold pred_at. Qed.
-
-    Definition infinite_trace tr :=
-      forall n, is_Some (after n tr).
-
-    Definition terminating_trace tr :=
-      ∃ n, after n tr = None.
-
-    Lemma terminating_trace_cons s ℓ tr:
-      terminating_trace tr -> terminating_trace (s -[ℓ]-> tr).
-    Proof. intros [n Hterm]. by exists (1+n). Qed.
-
-    Lemma infinite_trace_after n tr:
-      infinite_trace tr -> match after n tr with
-                          | None => False
-                          | Some tr' => infinite_trace tr'
-                          end.
-    Proof.
-      intros Hinf. have [tr' Htr'] := (Hinf n). rewrite Htr'.
-      intros m.
-      have Hnm := Hinf (n+m). rewrite after_sum' Htr' // in Hnm.
-    Qed.
-
-    Lemma infinite_cons s ℓ r:
-      infinite_trace (s -[ℓ]-> r) -> infinite_trace r.
-    Proof.
-      intros Hinf n. specialize (Hinf (1+n)).
-      rewrite (after_sum' _ 1) // in Hinf.
-    Qed.
-  End after.
 End fairness.
 
-Arguments ls_under {_ _}.
-Arguments ls_fuel {_ _}.
-Arguments ls_fuel_dom {_ _}.
-Arguments ls_mapping {_ _}.
-Arguments ls_mapping_dom {_ _}.
+Arguments LiveState : clear implicits.
+Arguments LiveModel : clear implicits.
+Arguments fair_model_model _ {_} _.
 
-Delimit Scope trace_scope with trace.
-Arguments tr_singl {_} {_}, _.
-Arguments tr_cons {_} {_} _ _ _%trace.
-Notation "⟨ s ⟩" := (tr_singl s) : trace_scope.
-Notation "s -[ ℓ ]->  r" := (tr_cons s ℓ r) (at level 33) : trace_scope.
-Open Scope trace.
-
-Section simulation.
-  Context {L1 L2 S1 S2: Type}.
-  Context (Rℓ: L1 -> L2 -> Prop) (Rs: S1 -> S2 -> Prop).
-  Context (trans1: S1 -> L1 -> S1 -> Prop).
-  Context (trans2: S2 -> L2 -> S2 -> Prop).
-
-  CoInductive traces_match : trace S1 L1 -> trace S2 L2 -> Prop :=
-  | trace_match_singl s1 s2: Rs s1 s2 -> traces_match ⟨ s1 ⟩ ⟨ s2 ⟩
-  | trace_match_cons s1 ℓ1 r1 s2 ℓ2 r2 : Rℓ ℓ1 ℓ2 -> Rs s1 s2 ->
-                                         trans1 s1 ℓ1 (trfirst r1) ->
-                                         trans2 s2 ℓ2 (trfirst r2) ->
-                                         traces_match r1 r2 ->
-                                         traces_match (s1 -[ℓ1]-> r1) (s2 -[ℓ2]-> r2).
-
-  Lemma traces_match_after tr1 tr2 n tr2':
-    traces_match tr1 tr2 ->
-    after n tr2 = Some tr2' ->
-    (exists tr1', after n tr1 = Some tr1' ∧ traces_match tr1' tr2').
-  Proof.
-    revert tr1 tr2.
-    induction n; intros tr1 tr2.
-    { simpl. intros. exists tr1. simplify_eq. done. }
-    move=> /= Hm Ha. destruct tr2 as [|s ℓ tr2''] eqn:Heq; first done.
-    destruct tr1; first by inversion Hm.
-    inversion Hm; simplify_eq. by eapply IHn.
-  Qed.
-
-  Lemma traces_match_first tr1 tr2:
-    traces_match tr1 tr2 ->
-    Rs (trfirst tr1) (trfirst tr2).
-  Proof. intros Hm. inversion Hm; done. Qed.
-
-End simulation.
-
-Section execs_and_traces.
-  Context {S L: Type}.
-
-  CoInductive exec_trace_match: finite_trace S L -> inflist (L * S) -> trace S L -> Prop :=
-  | exec_trace_match_singl ft s: trace_last ft = s -> exec_trace_match ft infnil ⟨s⟩
-  | exec_trace_match_cons ft s ℓ ift tr:
-      exec_trace_match (trace_extend ft ℓ s) ift tr ->
-      exec_trace_match ft (infcons (ℓ, s) ift) (trace_last ft -[ℓ]-> tr).
-
-  CoFixpoint to_trace (s: S) (il: inflist (L * S)) : trace S L :=
-    match il with
-    | infnil => ⟨ s ⟩
-    | infcons (ℓ, s') rest => s -[ℓ]-> (to_trace s' rest)
-    end.
-
-  Lemma to_trace_spec (fl: finite_trace S L) (il: inflist (L * S)):
-    exec_trace_match fl il (to_trace (trace_last fl) il).
-  Proof.
-    revert fl il. cofix CH. intros s il.
-    rewrite (trace_unfold_fold (to_trace _ il)). destruct il as [| [ℓ x]?]; simpl in *.
-    - by econstructor.
-    - econstructor. have ->: x = trace_last (trace_extend s ℓ x) by done.
-      apply CH.
-  Qed.
-
-  Lemma to_trace_singleton s (il: inflist (L * S)):
-    exec_trace_match (trace_singleton s) il (to_trace s il).
-  Proof. apply to_trace_spec. Qed.
-
-  CoFixpoint from_trace (tr: trace S L): inflist (L * S) :=
-    match tr with
-    | ⟨ s ⟩ => infnil
-    | s -[ℓ]-> tr' => infcons (ℓ, trfirst tr') (from_trace tr')
-    end.
-
-  Lemma from_trace_spec (fl: finite_trace S L) (tr: trace S L):
-    trace_last fl = trfirst tr ->
-    exec_trace_match fl (from_trace tr) tr.
-  Proof.
-    revert fl tr. cofix CH. intros fl tr Heq.
-    rewrite (inflist_unfold_fold (from_trace tr)). destruct tr; simpl in *.
-    - by econstructor.
-    - rewrite -Heq. econstructor. apply CH; done.
-  Qed.
-
-End execs_and_traces.
+Definition live_model_to_model : forall Λ M, LiveModel Λ M -> Model :=
+  λ Λ M lm, fair_model_model Λ lm.
+Coercion live_model_to_model : LiveModel >-> Model.
+Arguments live_model_to_model {_ _}.
 
 (* Basically, soundness of the logic and the lemmas above tell us that we have a program
    trace and a model trace which are related by traces_match labels_math!
@@ -393,8 +161,7 @@ End execs_and_traces.
 
 (* Definition of fairness for both kinds of traces *)
 
-
-Definition extrace {Λ} := trace (cfg Λ) (olocale Λ).
+Definition extrace Λ := trace (cfg Λ) (olocale Λ).
 
 Section exec_trace.
   Context {Λ : language}.
@@ -403,7 +170,7 @@ Section exec_trace.
   Definition locale_enabled (ζ : locale Λ) (c: cfg Λ) :=
     ∃ e, from_locale c.1 ζ = Some e ∧ to_val e = None.
 
-  Definition fair_ex ζ (extr: @extrace Λ): Prop :=
+  Definition fair_ex ζ (extr: extrace Λ): Prop :=
     forall n, pred_at extr n (λ c _, locale_enabled ζ c) ->
          ∃ m, pred_at extr (n+m) (λ c _, ¬locale_enabled ζ c)
               ∨ pred_at extr (n+m) (λ _ otid, otid = Some (Some ζ)).
@@ -424,7 +191,7 @@ Section exec_trace.
     fair_ex tid (c -[tid']-> r) -> fair_ex tid r.
   Proof. intros H. by eapply (fair_ex_after tid (c -[tid']-> r) r 1). Qed.
 
-  CoInductive extrace_valid: extrace (Λ := Λ) -> Prop :=
+  CoInductive extrace_valid: extrace Λ -> Prop :=
   | extrace_valid_singleton c: extrace_valid ⟨c⟩
   | extrace_valid_cons c oζ tr:
       locale_step c oζ (trfirst tr) ->
@@ -443,7 +210,7 @@ Section exec_trace.
     - apply CH; eauto. econstructor; try done. by destruct iex as [|[??]?].
   Qed.
 
-  Lemma from_trace_preserves_validity (extr: extrace) ex:
+  Lemma from_trace_preserves_validity (extr: extrace Λ) ex:
     extrace_valid extr ->
     valid_exec ex ->
     trace_last ex = trfirst extr ->
@@ -456,7 +223,7 @@ Section exec_trace.
       by econstructor.
   Qed.
 
-  Lemma from_trace_preserves_validity_singleton (extr: extrace):
+  Lemma from_trace_preserves_validity_singleton (extr: extrace Λ):
     extrace_valid extr ->
     valid_inf_exec (trace_singleton (trfirst extr)) (from_trace extr).
   Proof.
@@ -465,17 +232,14 @@ Section exec_trace.
 
 End exec_trace.
 
-
-Definition auxtrace {Λ: language} {M: FairModel} := trace (@LiveState Λ M) (@FairLabel Λ M.(fmrole)).
+Definition auxtrace `(LM: LiveModel Λ M) := trace LM.(lm_ls) LM.(lm_lbl).
 
 Section aux_trace.
-  Context {Λ: language}.
-  Context {M: FairModel}.
-  Context {LM: LiveModel Λ M}.
+  Context `{LM: LiveModel Λ M}.
 
-  Definition role_enabled ρ (δ: @LiveState Λ M) := ρ ∈ M.(live_roles) δ.
+  Definition role_enabled ρ (δ: LiveState Λ M) := ρ ∈ M.(live_roles) δ.
 
-  Definition fair_aux ρ (auxtr: auxtrace): Prop  :=
+  Definition fair_aux ρ (auxtr: auxtrace LM): Prop  :=
     forall n, pred_at auxtr n (λ δ _, role_enabled ρ δ) ->
          ∃ m, pred_at auxtr (n+m) (λ δ _, ¬role_enabled ρ δ)
               ∨ pred_at auxtr (n+m) (λ _ ℓ, ∃ tid, ℓ = Some (Take_step ρ tid)).
@@ -492,18 +256,18 @@ Section aux_trace.
     exists (p). by rewrite <-Nat.add_assoc, ->!(pred_at_sum _ n), Hafter in Hp.
   Qed.
 
-  CoInductive auxtrace_valid: @auxtrace Λ M -> Prop :=
+  CoInductive auxtrace_valid: auxtrace LM -> Prop :=
   | auxtrace_valid_singleton δ: auxtrace_valid ⟨δ⟩
   | auxtrace_valid_cons δ ℓ tr:
-      ls_trans (LM.(fuel_limit)) δ ℓ (trfirst tr) ->
+      LM.(lm_ls_trans) δ ℓ (trfirst tr) ->
       auxtrace_valid tr →
       auxtrace_valid (δ -[ℓ]-> tr).
 
-  Lemma auxtrace_valid_forall (tr: auxtrace) :
+  Lemma auxtrace_valid_forall (tr: auxtrace LM) :
     auxtrace_valid tr ->
     ∀ n, match after n tr with
          | Some ⟨ _ ⟩ | None => True
-         | Some (δ -[ℓ]-> tr') => ls_trans (LM.(fuel_limit)) δ ℓ (trfirst tr')
+         | Some (δ -[ℓ]-> tr') => LM.(lm_ls_trans) δ ℓ (trfirst tr')
          end.
   Proof.
     intros Hval n. revert tr Hval. induction n as [|n]; intros tr Hval;
@@ -514,116 +278,38 @@ Section aux_trace.
 
 End aux_trace.
 
-(* Adapted from Arthur Azevedo De Amorim *)
-Section lex_ind.
- Section Lexicographic.
-
-   Variables (A B : Type) (leA : relation A) (leB : relation B).
-
-   Inductive lexprod : A * B -> A * B -> Prop :=
-   | left_lex  : forall x x' y y', leA x x' -> lexprod (x, y) (x', y')
-   | right_lex : forall x y y',    leB y y' -> lexprod (x, y) (x, y').
-
-   Theorem wf_trans :
-     transitive _ leA ->
-     transitive _ leB ->
-     transitive _ lexprod.
-   Proof.
-     intros tA tB [x1 y1] [x2 y2] [x3 y3] H.
-     inversion H; subst; clear H.
-     - intros H.
-       inversion H; subst; clear H; apply left_lex; now eauto.
-    - intros H.
-    inversion H; subst; clear H.
-    + now apply left_lex.
-    + now apply right_lex; eauto.
-    Qed.
-
-    Theorem wf_lexprod :
-    well_founded leA ->
-    well_founded leB ->
-    well_founded lexprod.
-    Proof.
-      intros wfA wfB [x y]. generalize dependent y.
-      induction (wfA x) as [x _ IHx]; clear wfA.
-      intros y.
-      induction (wfB y) as [y _ IHy]; clear wfB.
-      constructor.
-      intros [x' y'] H.
-      now inversion H; subst; clear H; eauto.
-    Qed.
-
- End Lexicographic.
-
- Definition lt_lex : relation (nat * nat) := fun '(x, y) '(x', y') =>
-                                            x < x' ∨ (x = x' ∧ y <= y').
-
- #[global] Instance lt_lex_partial_order : @PartialOrder (nat * nat) lt_lex.
- Proof.
-   constructor.
-   + constructor.
-     * move=> [x y]. right; split; reflexivity.
-     * move=> [x1 y1] [x2 y2] [x3 y3] [H1|H1] [H2|H2]; unfold lt_lex; lia.
-   + move=> [x1 y1] [x2 y2] [?|[??]] [H2|[??]]; f_equal; try lia.
- Qed.
-
- Definition myrel : relation (nat * nat) :=
-    lexprod _ _ lt lt.
-
- Lemma lex_ind:
-   ∀ (n : nat*nat) (P : nat*nat → Prop),
-     (∀ n0 : nat*nat, (∀ m : nat*nat, (strict lt_lex) m n0 → P m) → P n0) → P n.
- Proof.
-   assert (well_founded myrel) as Hwf.
-   { apply wf_lexprod; apply lt_wf. }
-   induction n using (well_founded_ind Hwf).
-   intros P HI. apply HI =>//. intros m [Ha Hb].
-   apply H =>//. destruct n as [n1 n2]; destruct m as [m1 m2].
-   unfold strict, lt_lex in *.
-   destruct Ha as [Ha | [Ha1 Ha2]].
-   - constructor 1. done.
-    - rewrite Ha1. constructor 2. lia.
- Qed.
-
-End lex_ind.
-
 Ltac SS :=
   epose proof ls_fuel_dom;
   (* epose proof ls_mapping_dom; *)
   set_solver.
 
+Definition live_tids `{LM:LiveModel Λ M} `{EqDecision (locale Λ)}
+           (c : cfg Λ) (δ : LM.(lm_ls)) : Prop :=
+  (∀ ρ ζ, δ.(ls_mapping (Λ := Λ)) !! ρ = Some ζ -> is_Some (from_locale c.1 ζ)) ∧
+  ∀ ζ e, from_locale c.1 ζ = Some e -> (to_val e ≠ None) ->
+         ∀ ρ, δ.(ls_mapping) !! ρ ≠ Some ζ.
+
+Definition exaux_traces_match `{LM:LiveModel Λ M} `{EqDecision (locale Λ)} :
+  extrace Λ → auxtrace LM → Prop :=
+  traces_match labels_match
+               live_tids
+               locale_step
+               LM.(lm_ls_trans).
+
 Section fairness_preserved.
-  Context {M: FairModel}.
-  Context {Λ: language}.
-  Context {LM: LiveModel Λ M}.
+  Context `{LM: LiveModel Λ M}.
   Context `{Countable (locale Λ)}.
 
-  Definition live_tids (c: cfg Λ) (δ: LiveState M): Prop :=
-    (∀ ρ ζ, δ.(ls_mapping (Λ := Λ)) !! ρ = Some ζ -> is_Some (from_locale c.1 ζ)) ∧
-    ∀ ζ e, from_locale c.1 ζ = Some e -> (to_val e ≠ None) ->
-             ∀ ρ, δ.(ls_mapping) !! ρ ≠ Some ζ.
-
-  Notation exaux_traces_match :=
-    (@traces_match (olocale Λ)
-                   (LM.(mlabel))
-                   (cfg Λ)
-                   (LiveState M)
-                   labels_match
-                   live_tids
-                   locale_step
-                   (ls_trans LM.(fuel_limit))
-    ).
-
-  Lemma exaux_preserves_validity extr auxtr:
+  Lemma exaux_preserves_validity extr (auxtr : auxtrace LM):
     exaux_traces_match extr auxtr ->
-    (@auxtrace_valid _ _ LM) auxtr.
+    auxtrace_valid auxtr.
   Proof.
     revert extr auxtr. cofix CH. intros extr auxtr Hmatch.
     inversion Hmatch; first by constructor.
     constructor =>//. by eapply CH.
   Qed.
 
-  Lemma exaux_preserves_termination extr auxtr:
+  Lemma exaux_preserves_termination extr (auxtr : auxtrace LM) :
     exaux_traces_match extr auxtr ->
     terminating_trace auxtr ->
     terminating_trace extr.
@@ -641,7 +327,7 @@ Section fairness_preserved.
     eapply IHn =>//.
   Qed.
 
-  Lemma traces_match_labels {tid ℓ c δ rex raux}:
+  Lemma traces_match_labels tid ℓ c δ rex (raux : auxtrace LM) :
     exaux_traces_match (c -[Some tid]-> rex) (δ -[ℓ]-> raux) ->
     ((∃ ρ, ℓ = Take_step ρ tid) ∨ (ℓ = Silent_step tid)).
   Proof.
@@ -649,11 +335,11 @@ Section fairness_preserved.
     destruct ℓ; eauto; inversion Hlab; simplify_eq; eauto.
   Qed.
 
-  Lemma mapping_live_role (δ: LiveState M) ρ:
+  Lemma mapping_live_role (δ: LiveState Λ M) ρ:
     ρ ∈ M.(live_roles) δ ->
     is_Some (ls_mapping (Λ := Λ) δ !! ρ).
   Proof. rewrite -elem_of_dom ls_same_doms. SS. Qed.
-  Lemma fuel_live_role (δ: LiveState M) ρ:
+  Lemma fuel_live_role (δ: LiveState Λ M) ρ:
     ρ ∈ M.(live_roles) δ ->
     is_Some (ls_fuel (Λ := Λ) δ !! ρ).
   Proof. rewrite -elem_of_dom. SS. Qed.
@@ -661,7 +347,7 @@ Section fairness_preserved.
   Local Hint Resolve mapping_live_role: core.
   Local Hint Resolve fuel_live_role: core.
 
-  Lemma match_locale_enabled extr auxtr ζ ρ:
+  Lemma match_locale_enabled (extr : extrace Λ) (auxtr : auxtrace LM) ζ ρ:
     exaux_traces_match extr auxtr ->
     ls_mapping (trfirst auxtr) !! ρ = Some ζ ->
     locale_enabled ζ (trfirst extr).
@@ -674,23 +360,10 @@ Section fairness_preserved.
     have Hv: Some v ≠ None by []. by specialize (Hneqloc Hv ρ).
   Qed.
 
-  Lemma pred_first_aux (tr: auxtrace) (P: @LiveState Λ M -> Prop):
-    match tr with
-    | ⟨ s ⟩ | s -[ _ ]-> _ => P s
-    end <-> P (trfirst tr).
-  Proof. destruct tr; done. Qed.
-
-  Lemma pred_first_ex (tr: extrace) (P: cfg Λ -> Prop):
-    match tr with
-    | ⟨ s ⟩ | s -[ _ ]-> _ => P s
-    end <-> P (trfirst tr).
-  Proof. destruct tr; done. Qed.
-
   Local Hint Resolve match_locale_enabled: core.
-  Local Hint Resolve pred_first_aux: core.
-  Local Hint Resolve pred_first_ex: core.
+  Local Hint Resolve pred_first_trace: core.
 
-  Definition fairness_induction_stmt ρ fm f m ζ extr auxtr δ c :=
+  Definition fairness_induction_stmt ρ fm f m ζ extr (auxtr : auxtrace LM) δ c :=
       (infinite_trace extr ->
        (forall ζ, fair_ex ζ extr) ->
        fm = (f, m) ->
@@ -702,11 +375,11 @@ Section fairness_preserved.
       ∃ M, pred_at auxtr M (λ δ _, ¬role_enabled ρ δ)
            ∨ pred_at auxtr M (λ _ ℓ, ∃ ζ0, ℓ = Some (Take_step ρ ζ0))).
 
-  Local Lemma case1 ρ f m (extr' : @extrace Λ) auxtr' δ ℓ :
+  Local Lemma case1 ρ f m (extr' : extrace Λ) (auxtr' : auxtrace LM) δ ℓ :
     (∀ m0 : nat * nat,
          strict lt_lex m0 (f, m)
-         → ∀ (f m: nat) (ζ: locale Λ) (extr : extrace) (auxtr : auxtrace)
-             (δ : LiveState M) (c : cfg Λ), fairness_induction_stmt ρ m0 f m ζ extr auxtr δ c) ->
+         → ∀ (f m: nat) (ζ: locale Λ) (extr : extrace Λ) (auxtr : auxtrace LM)
+             (δ : LiveState Λ M) (c : cfg Λ), fairness_induction_stmt ρ m0 f m ζ extr auxtr δ c) ->
     (ρ ∈ dom (ls_fuel (trfirst auxtr')) → oless (ls_fuel (trfirst auxtr') !! ρ) (ls_fuel δ !! ρ)) ->
     exaux_traces_match extr' auxtr' ->
     infinite_trace extr' ->
@@ -729,11 +402,11 @@ Section fairness_preserved.
 
         have Hloc'en: pred_at extr' 0 (λ (c : cfg Λ) (_ : option (olocale Λ)),
                           locale_enabled ζ' c).
-        { rewrite /pred_at /= pred_first_ex. eauto. }
+        { rewrite /pred_at /= pred_first_trace. eauto. }
 
         have [p Hp] := (Hfair ζ' 0 Hloc'en).
-        have [P Hind] : ∃ M0 : nat, pred_at auxtr' M0 (λ (δ0 : LiveState M) _, ¬ role_enabled ρ δ0)
-                                  ∨ pred_at auxtr' M0 (λ (_ : LiveState M) ℓ, ∃ ζ0, ℓ = Some (Take_step ρ ζ0)).
+        have [P Hind] : ∃ M0 : nat, pred_at auxtr' M0 (λ (δ0 : LiveState Λ M) _, ¬ role_enabled ρ δ0)
+                                  ∨ pred_at auxtr' M0 (λ (_ : LiveState Λ M) ℓ, ∃ ζ0, ℓ = Some (Take_step ρ ζ0)).
         { eapply (IH _ _ _ p _ extr'); eauto.
           Unshelve. unfold strict, lt_lex. specialize (Hdec ltac:(by eapply elem_of_dom_2)). lia. }
         exists (1+P). rewrite !pred_at_sum. simpl. done.
@@ -744,7 +417,7 @@ Section fairness_preserved.
     Qed.
 
   Lemma fairness_preserved_ind ρ:
-    ∀ fm f m ζ (extr: @extrace Λ) (auxtr: auxtrace) δ c,
+    ∀ fm f m ζ (extr: extrace Λ) (auxtr: auxtrace LM) δ c,
       fairness_induction_stmt ρ fm f m ζ extr auxtr δ c.
   Proof.
     induction fm as [fm IH] using lex_ind.
@@ -758,7 +431,7 @@ Section fairness_preserved.
     { exists 0. left. unfold pred_at. simpl. intros contra. eauto. }
     destruct (decide (Some ζ = ζ')) as [Hζ|Hζ].
     - rewrite <- Hζ in *.
-      destruct (traces_match_labels Htm) as [[ρ' ->]| ->]; last first.
+      destruct (traces_match_labels _ _ _ _ _ _ Htm) as [[ρ' ->]| ->]; last first.
       + inversion Htm as [|s1 ℓ1 r1 s2 ℓ2 r2 Hl Hs Hts Hls Hmatchrest]; simplify_eq.
         unfold ls_trans in Hls.
         destruct Hls as (? & Hlsdec & Hlsincr).
@@ -819,7 +492,7 @@ Section fairness_preserved.
 
         unfold fair_ex in *.
         have Hζ'en: pred_at extr' 0 (λ (c : cfg Λ) _, locale_enabled ζ c).
-        { rewrite /pred_at /= pred_first_ex. inversion Htm; eauto. }
+        { rewrite /pred_at /= pred_first_trace. inversion Htm; eauto. }
         destruct m as [| m'].
         { rewrite -> !pred_at_0 in Hexen. destruct Hexen as [Hexen|Hexen].
           - exfalso. apply Hexen. unfold locale_enabled. by eapply (match_locale_enabled _ _ _ _ Htm).
@@ -859,9 +532,9 @@ Section fairness_preserved.
 
         unfold fair_ex in *.
         have: pred_at extr' 0 (λ c _, locale_enabled ζ'' c).
-        { rewrite /pred_at /= pred_first_ex. inversion Htm; eauto. }
+        { rewrite /pred_at /= pred_first_trace. inversion Htm; eauto. }
         have Hζ'en: pred_at extr' 0 (λ c _, locale_enabled ζ'' c).
-        { rewrite /pred_at /= pred_first_ex. inversion Htm; eauto. }
+        { rewrite /pred_at /= pred_first_trace. inversion Htm; eauto. }
         have [p Hp] := (Hfair' ζ'' 0 Hζ'en).
         have [P Hind] : ∃ M0 : nat, pred_at auxtr' M0 (λ δ0 _, ¬ role_enabled ρ δ0)
                         ∨ pred_at auxtr' M0 (λ _ ℓ, ∃ ζ0, ℓ = Some (Take_step ρ ζ0)).
@@ -870,7 +543,7 @@ Section fairness_preserved.
         exists (1+P). rewrite !pred_at_sum. simpl. done.
   Qed.
 
-  Theorem fairness_preserved (extr: @extrace Λ) (auxtr: auxtrace):
+  Theorem fairness_preserved (extr: extrace Λ) (auxtr: auxtrace LM):
     infinite_trace extr ->
     exaux_traces_match extr auxtr ->
     (forall ζ, fair_ex ζ extr) -> (forall ρ, fair_aux ρ auxtr).
@@ -905,11 +578,13 @@ Section fairness_preserved.
                 | [H: P |- _] => inversion H; clear H; simplify_eq
                                           end.
 
+  (* TODO: Why do we need explicit [LM] here? *)
   Definition valid_state_evolution_fairness
              (extr : execution_trace Λ) (auxtr : auxiliary_trace LM) :=
     match extr, auxtr with
     | (extr :tr[oζ]: (es, σ)), auxtr :tr[ℓ]: δ =>
-        labels_match oζ ℓ ∧ ls_trans LM.(fuel_limit) (trace_last auxtr) ℓ δ ∧ tids_smaller es δ
+        labels_match (LM:=LM) oζ ℓ ∧ LM.(lm_ls_trans) (trace_last auxtr) ℓ δ ∧
+        tids_smaller es δ
     | _, _ => True
     end.
 
@@ -918,16 +593,17 @@ Section fairness_preserved.
              (extr : execution_trace Λ) (auxtr : auxiliary_trace LM) :=
     valid_state_evolution_fairness extr auxtr ∧ φ extr auxtr.
 
+  (* TODO: Why do we need explicit [LM] here? *)
   Lemma valid_inf_system_trace_implies_traces_match
         (φ: execution_trace Λ -> auxiliary_trace LM -> Prop)
-        ex atr iex iatr progtr auxtr:
+        ex atr iex iatr progtr (auxtr : auxtrace LM):
     (forall (ex: execution_trace Λ) (atr: auxiliary_trace LM),
-        φ ex atr -> live_tids (trace_last ex) (trace_last atr)) ->
+        φ ex atr -> live_tids (LM:=LM) (trace_last ex) (trace_last atr)) ->
     (forall (ex: execution_trace Λ) (atr: auxiliary_trace LM),
         φ ex atr -> valid_state_evolution_fairness ex atr) ->
     exec_trace_match ex iex progtr ->
     exec_trace_match atr iatr auxtr ->
-    @valid_inf_system_trace _ LM φ ex atr iex iatr ->
+    valid_inf_system_trace φ ex atr iex iatr ->
     exaux_traces_match progtr auxtr.
   Proof.
     intros Hφ1 Hφ2.
@@ -935,86 +611,27 @@ Section fairness_preserved.
     intros ex atr iex iatr auxtr progtr Hem Ham Hval.
     inversion Hval as [?? Hphi |ex' atr' c [? σ'] δ' iex' iatr' oζ ℓ Hphi [=] ? Hinf]; simplify_eq.
     - inversion Hem; inversion Ham. econstructor; eauto.
-      pose proof (Hφ1 ex atr Hphi). congruence.
+      pose proof (Hφ1 ex atr Hphi).
+      by simplify_eq.
     - inversion Hem; inversion Ham. subst.
       pose proof (valid_inf_system_trace_inv _ _ _ _ _ Hinf) as Hphi'.
       destruct (Hφ2 (ex :tr[ oζ ]: (l, σ')) (atr :tr[ ℓ ]: δ') Hphi') as (?&?&?).
-      econstructor; eauto.
+      econstructor.
+      + eauto.
+      + eauto.
       + match goal with
         | [H: exec_trace_match _ iex' _ |- _] => inversion H; clear H; simplify_eq
         end; done.
       + match goal with
         | [H: exec_trace_match _ iatr' _ |- _] => inversion H; clear H; simplify_eq
         end; done.
+      + eapply IH; eauto.
   Qed.
 End fairness_preserved.
 
-#[global] Program Instance add_monoid: Monoid Nat.add :=
-  {| monoid_unit := 0 |}.
-Next Obligation. intros ???. apply Nat.add_assoc. Qed.
-Next Obligation. intros ??. apply Nat.add_comm. Qed.
-Next Obligation. intros ?. done. Qed.
-
-Section addition_monoid.
-  Context `{Countable K}.
-
-  Lemma big_addM_leq_forall (X Y: gmap K nat):
-    (∀ k, k ∈ dom X -> oleq (X !! k) (Y !! k)) ->
-    ([^ Nat.add map] k ↦ x ∈ X, x) ≤ ([^ Nat.add map] k ↦ y ∈ Y, y).
-  Proof.
-    revert Y.
-    induction X as [|k v X HXk IH] using map_ind.
-    { intros Y Hx. rewrite big_opM_empty /=. lia. }
-    intros Y Hx. rewrite big_opM_insert //.
-    have Hol: oleq (<[k:=v]> X !! k) (Y !! k) by apply Hx; set_solver.
-    rewrite lookup_insert in Hol.
-    destruct (Y!!k) as [v'|] eqn:Heq; last done.
-    rewrite (big_opM_delete _ Y k v') //.
-    apply plus_le_compat=>//.
-    apply IH=> k' Hin.
-    have ?: k ≠ k'.
-    { intros ->. apply elem_of_dom in Hin. rewrite HXk in Hin. by destruct Hin. }
-    rewrite -(lookup_insert_ne X k k' v) // (lookup_delete_ne Y k) //.
-    apply Hx. set_solver.
-  Qed.
-End addition_monoid.
-
-Section dec_unless.
-  Context {St S' L L': Type}.
-  Context (Us: St -> S').
-  Context (Ul: L -> option L').
-
-  Definition dec_unless Ψ (tr: trace St L) :=
-    ∀ n, match after n tr with
-         | Some ⟨ _ ⟩ | None => True
-         | Some (s -[ℓ]-> tr') =>
-           (∃ ℓ', Ul ℓ = Some ℓ') ∨
-           (Ψ (trfirst tr') < Ψ s ∧ Us s = Us (trfirst tr'))
-         end.
-
-  Lemma dec_unless_next Ψ s ℓ tr (Hdec: dec_unless Ψ (s -[ℓ]-> tr)): dec_unless Ψ tr.
-  Proof.
-    intros n. specialize (Hdec (n+1)). rewrite (after_sum 1) // in Hdec.
-  Qed.
-
-End dec_unless.
-
 Section fuel_dec_unless.
-  Context `{Mdl: FairModel}.
-  Context `{Λ: language}.
   Context `{LM: LiveModel Λ Mdl}.
   Context `{Countable (locale Λ)}.
-
-  Notation exaux_traces_match :=
-    (@traces_match (olocale Λ)
-                   LM.(mlabel)
-                   (cfg Λ)
-                   (LiveState Mdl)
-                   labels_match
-                   live_tids
-                   locale_step
-                   (ls_trans LM.(fuel_limit))
-    ).
 
   Definition Ul (ℓ: LM.(mlabel)) :=
     match ℓ with
@@ -1022,12 +639,12 @@ Section fuel_dec_unless.
     | _ => None
     end.
 
-  Definition Ψ (δ: LiveState Mdl) :=
+  Definition Ψ (δ: LiveState Λ Mdl) :=
     size δ.(ls_fuel) + [^ Nat.add map] ρ ↦ f ∈ δ.(ls_fuel (Λ := Λ)), f.
 
-  Lemma fuel_dec_unless (extr: extrace) (auxtr: auxtrace) :
+  Lemma fuel_dec_unless (extr: extrace Λ) (auxtr: auxtrace LM) :
     (∀ c c', locale_step (Λ := Λ) c None c' -> False) ->
-    exaux_traces_match extr auxtr ->
+    exaux_traces_match (LM:=LM) extr auxtr ->
     dec_unless ls_under Ul Ψ auxtr.
   Proof.
     intros Hcl Hval n. revert extr auxtr Hval. induction n; intros extr auxtr Hval; last first.
@@ -1077,219 +694,18 @@ Section fuel_dec_unless.
   Qed.
 End fuel_dec_unless.
 
-Section destuttering.
-  Context {St S' L L': Type}.
-  Context (Us: St -> S').
-  Context (Ul: L -> option L').
-
-  Inductive upto_stutter_ind (upto_stutter_coind: trace St L -> trace S' L' -> Prop):
-    trace St L -> trace S' L' -> Prop :=
-  | upto_stutter_singleton s:
-      upto_stutter_ind upto_stutter_coind ⟨s⟩ ⟨Us s⟩
-  | upto_stutter_stutter btr str s ℓ:
-      Ul ℓ = None ->
-      (* (Us s = Us (trfirst btr) -> (or something like this...?) *)
-      Us s = Us (trfirst btr) ->
-      Us s = trfirst str ->
-      upto_stutter_ind upto_stutter_coind btr str ->
-      upto_stutter_ind upto_stutter_coind (s -[ℓ]-> btr) str
-  | upto_stutter_step btr str s ℓ s' ℓ':
-      Us s = s' ->
-      Ul ℓ = Some ℓ' ->
-      upto_stutter_coind btr str ->
-      upto_stutter_ind upto_stutter_coind (s -[ℓ]-> btr) (s' -[ℓ']-> str).
-
-  Definition upto_stutter := paco2 upto_stutter_ind bot2.
-
-  Lemma upto_stutter_mono :
-    monotone2 (upto_stutter_ind).
-  Proof.
-    unfold monotone2. intros x0 x1 r r' IN LE.
-    induction IN; try (econstructor; eauto; done).
-  Qed.
-  Hint Resolve upto_stutter_mono : paco.
-
-  Lemma upto_stutter_after {btr str} n {str'}:
-    upto_stutter btr str ->
-    after n str = Some str' ->
-    ∃ n' btr', after n' btr = Some btr' ∧ upto_stutter btr' str'.
-  Proof.
-    have Hw: ∀ (P: nat -> Prop), (∃ n, P (S n)) -> (∃ n, P n).
-    { intros P [x ?]. by exists (S x). }
-    revert btr str str'. induction n as [|n IH]; intros btr str str' Hupto Hafter.
-    { injection Hafter => <-. clear Hafter. exists 0, btr. done. }
-    revert str' Hafter. punfold Hupto. induction Hupto as
-        [s|btr str s ℓ HUl HUs1 HUs2 Hind IHH|btr str s ℓ s' ℓ' ?? Hind].
-    - intros str' Hafter. done.
-    - intros str' Hafter.
-      apply Hw. simpl. by apply IHH.
-    - intros str' Hafter. simpl in Hafter.
-      apply Hw. simpl. eapply IH =>//.
-      by destruct Hind.
-  Qed.
-
-  Lemma upto_stutter_after_None {btr str} n:
-    upto_stutter btr str ->
-    after n str = None ->
-    ∃ n', after n' btr = None.
-  Proof.
-    have Hw: ∀ (P: nat -> Prop), (∃ n, P (S n)) -> (∃ n, P n).
-    { intros P [x ?]. by exists (S x). }
-    revert btr str. induction n as [|n IH]; intros btr str Hupto Hafter.
-    { exists 0. done. }
-    revert Hafter. punfold Hupto. induction Hupto as
-        [s|btr str s ℓ HUl HUs1 HUs2 Hind IHH|btr str s ℓ s' ℓ' ?? Hind].
-    - intros Hafter. by exists 1.
-    - intros Hafter.
-      apply Hw. simpl. by apply IHH.
-    - intros Hafter. simpl in Hafter.
-      apply Hw. simpl. eapply IH =>//.
-      by destruct Hind.
-  Qed.
-
-  Program Fixpoint destutter_once_step N Ψ (btr: trace St L) :
-    Ψ (trfirst btr) < N →
-    dec_unless Us Ul Ψ btr →
-    S' + (S' * L' * { btr' : trace St L | dec_unless Us Ul Ψ btr'}) :=
-    match N as n return
-          Ψ (trfirst btr) < n →
-          dec_unless Us Ul Ψ btr →
-          S' + (S' * L' * { btr' : trace St L | dec_unless Us Ul Ψ btr'})
-    with
-    | O => λ Hlt _, False_rect _ (Nat.nlt_0_r _ Hlt)
-    | S N' =>
-      λ Hlt Hdec,
-      match btr as z return btr = z → S' + (S' * L' * { btr' : trace St L | dec_unless Us Ul Ψ btr'}) with
-      | tr_singl s => λ _, inl (Us s)
-      | tr_cons s l btr' =>
-        λ Hbtreq,
-        match Ul l as z return Ul l = z → S' + (S' * L' * { btr' : trace St L | dec_unless Us Ul Ψ btr'}) with
-        | Some l' => λ _, inr (Us s, l', exist _ btr' _)
-        | None => λ HUll, destutter_once_step N' Ψ btr' _ _
-        end eq_refl
-      end eq_refl
-    end.
-  Next Obligation.
-  Proof.
-    intros _ Ψ btr N' Hlt Hdec s l btr' -> l' HUll; simpl.
-    eapply dec_unless_next; done.
-  Qed.
-  Next Obligation.
-  Proof.
-    intros _ Ψ btr N' Hlt Hdec s l btr' -> HUll; simpl in *.
-    pose proof (Hdec 0) as [[? ?]|[? ?]]; [congruence|lia].
-  Qed.
-  Next Obligation.
-  Proof.
-    intros _ Ψ btr N' Hlt Hdec s l btr' -> HUll; simpl.
-    eapply dec_unless_next; done.
-  Qed.
-
-  CoFixpoint destutter_gen Ψ N (btr: trace St L) :
-    Ψ (trfirst btr) < N ->
-    dec_unless Us Ul Ψ btr → trace S' L' :=
-    λ Hlt Hdec,
-    match destutter_once_step N Ψ btr Hlt Hdec with
-    | inl s' => tr_singl s'
-    | inr (s', l', z) => tr_cons s' l' (destutter_gen Ψ  (S (Ψ (trfirst $ proj1_sig z)))
-                                                 (proj1_sig z) (Nat.lt_succ_diag_r _) (proj2_sig z))
-    end.
-
-  Definition destutter Ψ (btr: trace St L) :
-    dec_unless Us Ul Ψ btr → trace S' L' :=
-    λ Hdec,
-    destutter_gen Ψ (S (Ψ (trfirst btr))) btr (Nat.lt_succ_diag_r _) Hdec.
-
-  Lemma destutter_same_Us N Ψ btr Hlt Hdec:
-    match destutter_once_step N Ψ btr Hlt Hdec with
-    | inl s' | inr (s', _, _) => Us (trfirst btr) = s'
-    end.
-  Proof.
-    revert btr Hlt Hdec. induction N as [|N]; first lia.
-    intros btr Hlt Hdec. simpl.
-    destruct btr as [s|s ℓ btr']; first done.
-    generalize (destutter_once_step_obligation_1 Ψ (s -[ ℓ ]-> btr') N
-                Hlt Hdec s ℓ btr' eq_refl).
-    generalize (destutter_once_step_obligation_2 Ψ (s -[ ℓ ]-> btr') N Hlt Hdec s ℓ btr' eq_refl).
-    generalize (destutter_once_step_obligation_3 Ψ (s -[ ℓ ]-> btr') N Hlt Hdec s ℓ btr' eq_refl).
-    intros HunlessNone HltNone HdecSome.
-    destruct (Ul ℓ) as [ℓ'|] eqn:Heq; cbn; first done.
-    unfold dec_unless in Hdec.
-    destruct (Hdec 0) as [[??]|[? Hsame]]; first congruence.
-    rewrite Hsame. apply IHN.
-  Qed.
-
-  Lemma destutter_spec_ind N Ψ (btr: trace St L) (Hdec: dec_unless Us Ul Ψ btr)
-    (Hlt: Ψ (trfirst btr) < N):
-    upto_stutter btr (destutter_gen Ψ N btr Hlt Hdec).
-  Proof.
-    revert N btr Hlt Hdec.
-    pcofix CH. pfold.
-    induction N.
-    { intros; lia. }
-    intros btr Hlt Hdec.
-    rewrite (trace_unfold_fold (destutter_gen _ _ _ _ _)).
-    destruct btr as [s|s ℓ btr'].
-    { simpl in *. econstructor. }
-    cbn.
-    generalize (destutter_once_step_obligation_1 Ψ (s -[ ℓ ]-> btr') N
-                Hlt Hdec s ℓ btr' eq_refl).
-    generalize (destutter_once_step_obligation_2 Ψ (s -[ ℓ ]-> btr') N Hlt Hdec s ℓ btr' eq_refl).
-    generalize (destutter_once_step_obligation_3 Ψ (s -[ ℓ ]-> btr') N Hlt Hdec s ℓ btr' eq_refl).
-    intros HunlessNone HltNone HdecSome.
-    destruct (Ul ℓ) as [ℓ'|] eqn:Heq; cbn.
-    - econstructor 3 =>//. right. apply (CH (S (Ψ $ trfirst btr'))).
-    - econstructor 2=>//.
-      + destruct (Hdec 0) as [[??]|[??]];congruence.
-      + have ?: Us s = Us (trfirst btr').
-        { destruct (Hdec 0) as [[??]|[? Hsame]]; congruence. }
-        have HH := destutter_same_Us N Ψ btr' (HltNone eq_refl) (HunlessNone eq_refl).
-        destruct (destutter_once_step N Ψ btr' (HltNone eq_refl) (HunlessNone eq_refl)) as
-            [|[[??][??]]]eqn:Heq'; simpl in *; congruence.
-      + rewrite -trace_unfold_fold.
-        specialize (IHN btr' (HltNone eq_refl) (HunlessNone eq_refl)).
-        match goal with
-          [H : context[upto_stutter_ind]  |- ?Y] => let X := type of H in
-                          suffices <-: X <-> Y; first done
-        end.
-        f_equiv.
-        rewrite {1}(trace_unfold_fold (destutter_gen _ _ _ _ _)) /= -trace_unfold_fold //.
-  Qed.
-
-  Lemma destutter_spec Ψ (btr: trace St L) (Hdec: dec_unless Us Ul Ψ btr):
-    upto_stutter btr (destutter Ψ btr Hdec).
-  Proof. eapply destutter_spec_ind. Qed.
-
-  Lemma can_destutter Ψ (btr: trace St L) (Hdec: dec_unless Us Ul Ψ btr):
-    ∃ str, upto_stutter btr str.
-  Proof. exists (destutter Ψ btr Hdec). apply destutter_spec. Qed.
-
-End destuttering.
-
 Section destuttering_auxtr.
-  Context {Mdl: FairModel}.
-  Context {Λ: language}.
-  Context {LM: LiveModel Λ Mdl}.
+  Context `{LM: LiveModel Λ M}.
 
   Context `{Countable (locale Λ)}.
 
-  Notation exaux_traces_match :=
-    (@traces_match (olocale Λ)
-                   (LM.(mlabel))
-                   (cfg Λ)
-                   (LiveState Mdl)
-                   labels_match
-                   live_tids
-                   locale_step
-                   (ls_trans LM.(fuel_limit))
-    ).
-
+  (* Why is [LM] needed here? *)
   Definition upto_stutter_auxtr :=
-    upto_stutter (@ls_under Λ Mdl) (Ul (Mdl := Mdl) (Λ := Λ) (LM := LM)).
+    upto_stutter (ls_under (Λ:=Λ) (M:=M)) (Ul (LM := LM)).
 
   Lemma can_destutter_auxtr extr auxtr:
     (∀ c c', locale_step (Λ := Λ) c None c' -> False) ->
-    exaux_traces_match extr auxtr ->
+    exaux_traces_match (LM:=LM) extr auxtr ->
     ∃ mtr, upto_stutter_auxtr auxtr mtr.
   Proof.
     intros ??. eapply can_destutter.
@@ -1299,14 +715,12 @@ Section destuttering_auxtr.
 End destuttering_auxtr.
 
 Section model_traces.
-  Context {Mdl: FairModel}.
-  Context {Λ: language}.
-  Context {LM: LiveModel Λ Mdl}.
+  Context `{LM: LiveModel Λ M}.
   Context `{Countable (locale Λ)}.
 
-  Definition mtrace := trace Mdl (option Mdl.(fmrole)).
+  Definition mtrace := trace M (option M.(fmrole)).
 
-  Definition role_enabled_model ρ (s: Mdl) := ρ ∈ Mdl.(live_roles) s.
+  Definition role_enabled_model ρ (s: M) := ρ ∈ M.(live_roles) s.
 
   Definition fair_model_trace ρ (mtr: mtrace): Prop  :=
     forall n, pred_at mtr n (λ δ _, role_enabled_model ρ δ) ->
@@ -1350,16 +764,16 @@ Section model_traces.
   Hint Resolve mtrace_valid_mono : paco.
 
   Lemma upto_stutter_mono' :
-    monotone2 (upto_stutter_ind (@ls_under Λ Mdl) (@Ul Mdl Λ LM)).
+    monotone2 (upto_stutter_ind (ls_under (Λ:=Λ) (M:=M)) (Ul (LM:=LM))).
   Proof.
     unfold monotone2. intros x0 x1 r r' IN LE.
     induction IN; try (econstructor; eauto; done).
   Qed.
   Hint Resolve upto_stutter_mono' : paco.
 
-  Lemma upto_preserves_validity auxtr mtr:
-    upto_stutter_auxtr (LM := LM) auxtr mtr ->
-    auxtrace_valid (LM := LM) auxtr ->
+  Lemma upto_preserves_validity (auxtr : auxtrace LM) mtr:
+    upto_stutter_auxtr auxtr mtr ->
+    auxtrace_valid auxtr ->
     mtrace_valid mtr.
   Proof.
     revert auxtr mtr. pcofix CH. intros auxtr mtr Hupto Hval.
@@ -1383,24 +797,23 @@ End model_traces.
 Global Hint Resolve fair_model_trace_cons: core.
 Global Hint Resolve fair_model_trace_cons: core.
 
-Section upto_stutter_preserves_fairness_and_terminaison.
-  Context {Mdl: FairModel}.
-  Context {Λ: language}.
-  Context {LM: LiveModel Λ Mdl}.
-  Context `{Countable (locale Λ)}.
+Arguments mtrace : clear implicits.
 
+Section upto_stutter_preserves_fairness_and_termination.
+  Context `{LM: LiveModel Λ M}.
+  Context `{Countable (locale Λ)}.
 
   Notation upto_stutter_aux := (upto_stutter (ls_under (Λ := Λ)) (Ul (Λ := Λ) (LM := LM))).
 
   Lemma upto_stutter_mono'' : (* TODO fix this proliferation *)
-    monotone2 (upto_stutter_ind (@ls_under Λ Mdl) (@Ul Mdl Λ LM)).
+    monotone2 (upto_stutter_ind (ls_under (Λ:=Λ) (M:=M)) (Ul (LM:=LM))).
   Proof.
     unfold monotone2. intros x0 x1 r r' IN LE.
     induction IN; try (econstructor; eauto; done).
   Qed.
   Hint Resolve upto_stutter_mono' : paco.
 
-  Lemma upto_stutter_fairness_0 ρ auxtr (mtr: @mtrace Mdl):
+  Lemma upto_stutter_fairness_0 ρ auxtr (mtr: mtrace M):
     upto_stutter_aux auxtr mtr ->
     (* role_enabled_model ρ (trfirst mtr) -> *)
     (∃ n, pred_at auxtr n (λ δ _, ¬role_enabled (Λ := Λ) ρ δ)
@@ -1439,7 +852,7 @@ Section upto_stutter_preserves_fairness_and_terminaison.
             { destruct IH as [|]; done. }
     Qed.
 
-  Lemma upto_stutter_fairness auxtr (mtr: @mtrace Mdl):
+  Lemma upto_stutter_fairness (auxtr:auxtrace LM) (mtr: mtrace M):
     upto_stutter_aux auxtr mtr ->
     (∀ ρ, fair_aux ρ auxtr) ->
     (∀ ρ, fair_model_trace ρ mtr).
@@ -1462,7 +875,7 @@ Section upto_stutter_preserves_fairness_and_terminaison.
     exists m. rewrite !(pred_at_sum _ n) Heq //.
   Qed.
 
-  Lemma upto_stutter_finiteness auxtr (mtr: @mtrace Mdl):
+  Lemma upto_stutter_finiteness auxtr (mtr: mtrace M):
     upto_stutter_aux auxtr mtr ->
     terminating_trace mtr ->
     terminating_trace auxtr.
@@ -1472,23 +885,6 @@ Section upto_stutter_preserves_fairness_and_terminaison.
     eexists; done.
   Qed.
 
-End upto_stutter_preserves_fairness_and_terminaison.
-
-(* Classical *)
-
-Require Import Coq.Logic.Classical.
-Section infinite_or_finite.
-  Context {St L: Type}.
-
-  Lemma infinite_or_finite (tr: trace St L):
-    infinite_trace tr ∨ terminating_trace tr.
-  Proof.
-    destruct (classic (infinite_trace tr)) as [|Hni]; first by eauto.
-    rewrite /infinite_trace in Hni.
-    apply not_all_ex_not in Hni. destruct Hni as [n Hni%eq_None_not_Some].
-    by right; exists n.
-  Qed.
-
-End infinite_or_finite.
+End upto_stutter_preserves_fairness_and_termination.
 
 Global Hint Resolve mtrace_valid_mono : paco.
